---
title: "Calculus: Part 2 - All About Derivatives"
date: 2024-06-21 00:00:00 -0600
categories: [Math, Calculus]
tags: [math, calculus]
---
<script
  src="https://cdn.mathjax.org/mathjax/latest/MathJax.js?config=TeX-AMS-MML_HTMLorMML"
  type="text/javascript">
</script>

# Calculus
## Part 2 - All About Derivatives

### 2.1 - Basic Rules
There are basic patterns and rules when differentiating a function. The most famous example is the **power rule**, which is as follows.

$$(x^n)'=nx^{n-1}$$

The derivative of a sum of functions is the sum of the derivatives of each term:
$$(f+g)'=f'+g'$$

A **second derivative** is the derivative of a derivative. It can be represented like this:

$$\frac{d^2y}{dx^2}$$
or
$$f''(x)$$

Similarly, the 
$$n$$
th derivative can be represented like this:

$$\frac{d^ny}{dx^n}$$
or
$$f^{(n)}(x)$$

**Transcendental functions** are functions that canâ€™t be written as a power function (including radical and rational functions). These include exponential, logarithmic, and trigonometric functions. Each of them has unique derivatives:

$$(\sin x)'=\cos x$$

$$(\cos x)'=-\sin x$$

$$(e^x)'=e^x$$

$$(\ln x)'=1/x$$

### 2.2 - Product and Quotient Rules
There are special rules for dealing with products and quotients of functions such as 
$$x^2\sin x$$
. For the following rules, let's imagine that 
$$f$$
and
$$g$$
are functions.

The product rule for states that 
$$(f\cdot g)' = f'\cdot g +f \cdot g'$$
.

Meanwhile, the quotient rule states that
$$(\frac{f}{g})' = \frac{f'\cdot g -f \cdot g'}{g^2}$$

From what was covered so far, we can find the following derivative identities:

$$(\tan x)' = \sec ^2x$$

$$(\cot x)' = -\csc ^2x$$

$$(\sec x)' = \sec x \cdot \tan x$$

$$(\csc x)' = -\csc x \cdot \cot x$$

All the "co-" functions have negative derivatives that include the corresponding "co-" function.
### 2.3 - The Chain Rule
The **chain rule** is used for differentiating a composite function (in which there is a function inside of a function). An example of a composite function is 
$$\cos x^2$$
. The 
$$x^2$$
function is inside of the
$$\cos x$$
function. The chain rule states that

$$[f(g)]' = f'(g) \cdot g'$$
, where 
$$f$$
is the outside function and 
$$g$$
is the inside function. In other words, the derivative of a composite function is the derivative of the outside times the derivative of the inside.

Going back to our example, 
$$\cos x^2$$
, the derivative of cosine is negative sine, so the "derivative of the outside" is
$$-\sin x^2$$
. Now, the inside function is 
$$x^2$$
, whose derivative is 
$$2x$$
. So the derivative of 
$$\cos x^2$$
is 
$$-\sin (x^2) \cdot 2x$$
.

We are now able to find the derivative of any logarithmic function:

$$c^x=e^{x\ln(a)}=a^x\ln(a)$$
In this case, 
$$c$$
is a constant, so the product rule is not needed.

### 2.4 - Inverse Function Rule
The derivative of an inverse function, where the output becomes the input and vice versa, has its own special rule:

$$[f^{-1}]' = \frac{1}{f'(f^{-1})}$$

**Fun fact:** The derivative of an inverse function is the reciprocal of the slope of the original function. For example look at this table:

![Table](/images/calc-2-graph.PNG)

Let's say that
$$h(x)$$
was the inverse of
$$g(x)$$
. Then,
$$h'(4) = \frac{1}{g'(1)} = -\frac{1}{2} $$
. We can also find the identities of the inverse trigonometric functions:

$$(\sin^{-1} x)' = (\arcsin x)' = \frac{1}{\sqrt{1-x^2} } $$

$$(\cos^{-1} x)' = (\arccos x)' = -\frac{1}{\sqrt{1-x^2} } $$

$$(\tan^{-1} x)' = (\arctan x)' = \frac{1}{1+x^2} $$

<font size="5">Continued on part 3: Analyzing with Derivatives</font>